Add type scheme erasure and make erasure total
This was non-trivial because we have to use information about the arity
of the type scheme to determine when to call normal erasure. In
particular, for partial application such as

Definition alias : Type -> Type := option.

We have to eta expand alias before we can erase it with normal type
erasure, since `option` needs to be applied before it is a type. To
carry all the proofs through we thus need more information about arities
than we had previously, as we now need to know how many arguments are
expected.

Thus, flag_of_type changes significantly. It now returns a proof of
whether the type is convertible or not to a `conv_arity` record that
contains information about the arity: the domains, the universe (as
informational content), plus a proof that the type is convertible to the
arity created from these.

As a result we can now make erasure total since we now have the ability
to erase all constant declarations. Previously we were also failing on
axiomatic type schemes, however now the AST allows a type alias to have
no body to handle this when printing instead.

extraction/examples/ErasureTests.v
@@ -30,75 +30,74 @@ Record type_flag_squashed :=
     is_sort : bool;
     is_arity : bool }.
 
-Program Definition flag_of_type_program (p : Ast.program)
-  : result type_flag_squashed string :=
+Program Definition flag_of_type_program (p : Ast.program) : type_flag_squashed :=
   let p := fix_program_universes p in
   let Σ := trans_global_decls p.1 in
   let f := flag_of_type (empty_ext Σ) _ [] (trans p.2) _ in
-  ret {| is_logical := Erasure.is_logical f;
-         is_sort := if Erasure.is_sort f then true else false;
-         is_arity := if Erasure.is_arity f then true else false |}.
+  {| is_logical := Erasure.is_logical f;
+     is_sort := if Erasure.is_sort (conv_ar f) then true else false;
+     is_arity := if Erasure.is_arity (conv_ar f) then true else false |}.
 Next Obligation. Admitted.
 Next Obligation. Admitted.
 
 MetaCoq Quote Recursively Definition ex1 := Type.
 Example ex1_test :
   flag_of_type_program ex1 =
-  Ok {| is_logical := false; is_sort := true; is_arity := true |}.
+  {| is_logical := false; is_sort := true; is_arity := true |}.
 Proof. vm_compute. reflexivity. Qed.
 
 MetaCoq Quote Recursively Definition ex2 := nat.
 Example ex2_test :
   flag_of_type_program ex2 =
-  Ok {| is_logical := false; is_sort := false; is_arity := false |}.
+  {| is_logical := false; is_sort := false; is_arity := false |}.
 Proof. vm_compute. reflexivity. Qed.
 
 MetaCoq Quote Recursively Definition ex3 := (nat -> nat).
 Example ex3_test :
   flag_of_type_program ex3 =
-  Ok {| is_logical := false; is_sort := false; is_arity := false |}.
+  {| is_logical := false; is_sort := false; is_arity := false |}.
 Proof. vm_compute. reflexivity. Qed.
 
 MetaCoq Quote Recursively Definition ex4 := (forall A, A).
 Example ex4_test :
   flag_of_type_program ex4 =
-  Ok {| is_logical := false; is_sort := false; is_arity := false |}.
+  {| is_logical := false; is_sort := false; is_arity := false |}.
 Proof. vm_compute. reflexivity. Qed.
 
 MetaCoq Quote Recursively Definition ex5 := (Prop).
 Example ex5_test :
   flag_of_type_program ex5 =
-  Ok {| is_logical := true; is_sort := true; is_arity := true |}.
+  {| is_logical := true; is_sort := true; is_arity := true |}.
 Proof. vm_compute. reflexivity. Qed.
 
 MetaCoq Quote Recursively Definition ex5' := (forall n m: nat, Prop).
 Example ex5'_test :
   flag_of_type_program ex5' =
-  Ok {| is_logical := true; is_sort := false; is_arity := true |}.
+  {| is_logical := true; is_sort := false; is_arity := true |}.
 Proof. vm_compute. reflexivity. Qed.
 
 MetaCoq Quote Recursively Definition ex6 := (Prop -> Type).
 Example ex6_test :
   flag_of_type_program ex6 =
-  Ok {| is_logical := false; is_sort := false; is_arity := true |}.
+  {| is_logical := false; is_sort := false; is_arity := true |}.
 Proof. vm_compute. reflexivity. Qed.
 
 MetaCoq Quote Recursively Definition ex7 := (Type -> Prop).
 Example ex7_test :
   flag_of_type_program ex7 =
-  Ok {| is_logical := true; is_sort := false; is_arity := true |}.
+  {| is_logical := true; is_sort := false; is_arity := true |}.
 Proof. vm_compute. reflexivity. Qed.
 
 MetaCoq Quote Recursively Definition ex8 := (False).
 Example ex8_test :
   flag_of_type_program ex8 =
-  Ok {| is_logical := true; is_sort := false; is_arity := false |}.
+  {| is_logical := true; is_sort := false; is_arity := false |}.
 Proof. vm_compute. reflexivity. Qed.
 
 MetaCoq Quote Recursively Definition ex9 := (Fin.t 0 -> False).
 Example ex9_test :
   flag_of_type_program ex9 =
-  Ok {| is_logical := true; is_sort := false; is_arity := false |}.
+  {| is_logical := true; is_sort := false; is_arity := false |}.
 Proof. vm_compute. reflexivity. Qed.
 End flag_of_type_tests.
 
@@ -357,8 +356,7 @@ Proof. vm_compute. reflexivity. Qed.
 End erase_type_tests.
 
 Module erase_ind_arity_tests.
-Program Definition erase_arity_program (p : Ast.program)
-: list oib_type_var :=
+Program Definition erase_arity_program (p : Ast.program) : list type_var_info :=
   let p := fix_program_universes p in
   let Σ := trans_global_decls p.1 in
   erase_ind_arity (empty_ext Σ) _ [] (trans p.2) _.
@@ -594,3 +592,89 @@ Example IndWithIndex_test :
 "| ex14_ctor □" $>.
 Proof. vm_compute. reflexivity. Qed.
 End erase_ind_tests.
+
+Module erase_type_scheme_tests.
+Axiom assume_wellformed : forall {X}, X.
+Axiom does_not_happen : forall {X}, X.
+Definition erase_and_print_type_scheme (p : Ast.program) : string * string :=
+  let p := fix_program_universes p in
+  let Σ := trans_global_decls p.1 in
+  match trans p.2 with
+  | P.tConst kn _ =>
+    match lookup_env Σ kn with
+    | Some (P.ConstantDecl cst) =>
+      let r := erase_constant_decl
+                 (Σ, cst_universes cst) assume_wellformed
+                 cst assume_wellformed in
+      match r with
+      | inr (Some (tvars, bt)) =>
+        let tvars := map tvar_name tvars in
+        (erase_type_tests.print_type_vars tvars,
+         erase_type_tests.print_box_type Σ tvars bt)
+      | _ => does_not_happen
+      end
+    | _ => does_not_happen
+    end
+  | _ => does_not_happen
+  end.
+
+Definition nat_alias := nat.
+MetaCoq Quote Recursively Definition ex1 := nat_alias.
+Example ex1_test :
+  erase_and_print_type_scheme ex1 = ("", "nat").
+Proof. vm_compute. reflexivity. Qed.
+
+Definition list_nat := list nat.
+MetaCoq Quote Recursively Definition ex2 := list_nat.
+Example ex2_test :
+  erase_and_print_type_scheme ex2 = ("", "list nat").
+Proof. vm_compute. reflexivity. Qed.
+
+Definition list_alias T := list T.
+MetaCoq Quote Recursively Definition ex3 := list_alias.
+Example ex3_test :
+  erase_and_print_type_scheme ex3 = ("T", "list T").
+Proof. vm_compute. reflexivity. Qed.
+
+Definition list_alias_eta := list.
+MetaCoq Quote Recursively Definition ex4 := list_alias_eta.
+Example ex4_test :
+  (* Names are taken from arity when eta expanding *)
+  erase_and_print_type_scheme ex4 = ("A", "list A").
+Proof. vm_compute. reflexivity. Qed.
+
+Inductive anon_list : Type -> Type :=
+| anil : forall T, anon_list T
+| acons : forall T, T -> anon_list T -> anon_list T.
+
+Definition anon_list_alias_eta := anon_list.
+MetaCoq Quote Recursively Definition ex5 := anon_list_alias_eta.
+Example ex5_test :
+  erase_and_print_type_scheme ex5 = ("_", "anon_list _").
+Proof. vm_compute. reflexivity. Qed.
+
+Definition option_wrap T := option T.
+MetaCoq Quote Recursively Definition ex6 := option_wrap.
+Example ex6_test :
+  erase_and_print_type_scheme ex6 = ("T", "option T").
+Proof. vm_compute. reflexivity. Qed.
+
+Definition vector_wrap T n := Vector.t (option T) n.
+MetaCoq Quote Recursively Definition ex7 := vector_wrap.
+Example ex7_test :
+  erase_and_print_type_scheme ex7 = ("T n", "t (option T) 𝕋").
+Proof. vm_compute. reflexivity. Qed.
+
+Definition vector_wrap_eta T := Vector.t (option T).
+MetaCoq Quote Recursively Definition ex8 := vector_wrap_eta.
+Example ex8_test :
+  erase_and_print_type_scheme ex8 = ("T _", "t (option T) 𝕋").
+Proof. vm_compute. reflexivity. Qed.
+
+Fixpoint vector_wrap_fix T n := Vector.t (option T) n.
+MetaCoq Quote Recursively Definition ex9 := vector_wrap_fix.
+Example ex9_test :
+  erase_and_print_type_scheme ex9 = ("T n", "𝕋").
+Proof. vm_compute. reflexivity. Qed.
+
+End erase_type_scheme_tests.
